Fix scheduler to return result of main fiber.
The scheduler allocates a new reference to hold the eventual result. If
there is no next fiber in the run queue, then this reference is checked
to see if the main fiber has already exited. If it's not then the main
fiber must be blocked on something (maybe even diverged), so the
scheduler busy loops on checking if something is in the run queue.
When the fiber unblocks at some point, it will be placed into the run
queue and the scheduler can continue.

theories/case_studies/eio/eio.v
@@ -29,18 +29,17 @@ From iris.algebra Require Import excl_auth gset gmap agree csum frac excl.
 From iris.base_logic Require Import invariants.
 From iris.base_logic.lib Require Import iprop wsat saved_prop.
 From program_logic Require Import reasoning_rules.
-From case_studies Require Import list_lib .
 
 From case_studies.eio Require Import concurrent_queue cqs.
 
 (* ========================================================================== *)
 (** * Implementation of the Scheduler. *)
 
-Notation Fork state e := (InjL (Pair state e)) (only parsing).
+Notation Fork tlv e := (InjL (Pair tlv e)) (only parsing).
 Notation Suspend f := (InjR (InjL f)) (only parsing).
 Notation GetContext := (InjR (InjR #())) (only parsing).
 
-Notation Fork' state e := (InjLV (PairV state e)) (only parsing).
+Notation Fork' tlv e := (InjLV (PairV tlv e)) (only parsing).
 Notation Suspend' f := (InjRV (InjLV f)) (only parsing).
 Notation GetContext' := (InjRV (InjRV #())) (only parsing).
 
@@ -50,22 +49,40 @@ Notation Waiting ws := (InjR ws) (only parsing).
 Notation Done' y := (InjLV y) (only parsing).
 Notation Waiting' ws := (InjRV ws) (only parsing).
 
-Section implementation.
-  Context `{!heapGS Σ, !ListLib Σ}.
+Notation NONE := (InjL #()) (only parsing).
+Notation SOME x := (InjR x) (only parsing).
 
+Notation NONE' := (InjLV #()) (only parsing).
+Notation SOME' x := (InjRV x) (only parsing).
+
+Section implementation.
+  Context `{!heapGS Σ }.
+
+  Definition new_scheduler_result : val := (λ: <>,
+    ref NONE'
+  )%V.
   Definition new_promise : val := (λ: <>,
     ref (Waiting (cqs_new #()))
   )%V.
-  Definition new_fiber_state : val := (λ: <>,
-    ref #0
+  Definition new_context : val := (λ: "init",
+    ref "init"
   )%V.
-  Definition fork : val := (λ: "state" "f", do: (Fork "state" "f"))%V.
+  Definition fork : val := (λ: "tlv" "f", do: (Fork "tlv" "f"))%V.
   Definition suspend : val := (λ: "f", do: (Suspend "f"))%V.
   Definition get_context : val := (λ: <>, do: GetContext)%V.
+  
+  Definition yield : val := (λ: <>,
+    let: "register" := λ: "waker", "waker" #() in
+    suspend "register"
+  )%V.
 
-  Definition next : val := (λ: "q",
+  Definition next : val := (rec: "next" "res" "q" :=
     match: queue_pop "q" with
-      (* Empty *) InjL <> => #()
+      (* Empty *) InjL <> => 
+        match: Load "res" with
+          (* Not Done *) InjL <> => "next" "res" "q"
+        | (* Done *)     InjR <> => #() (* diverge *)
+        end
     | (* Nonempty *) InjR "f" => "f" #()
     end)%V.
 
@@ -82,10 +99,10 @@ Section implementation.
 
   (* fork a new fiber "f" and return a promise to get the result. *)
   Definition fork_promise : val := (λ: "f", 
-    let: "state" := get_context #() in
+    let: "tlv" := get_context #() in
     let: "p" := new_promise #() in
     let: "wrapped_f" := fork_wrap_f "f" "p" in
-    fork "state" "wrapped_f";;
+    fork "tlv" "wrapped_f";;
     "p")%V.
    
   Definition await_callback : val := (λ: "p" "ws", (λ: "waker", 
@@ -121,36 +138,42 @@ Section implementation.
         end
     end
   )%V.
+
+
+  Definition execute : val := (λ: "q" "result", rec: "execute" "context" "f" :=
+    deep-try: "f" #() with
+      effect (λ: "request" "k",
+        match: "request" with
+          (* Fork: *) InjL "contextf" =>
+            let: "new_context" := Fst "contextf" in 
+            let: "f" := Snd "contextf" in
+            queue_push "q" (λ: <>, "k" #());;
+            "execute" "new_context" "f"
+        | (* Suspend/GetContext: *) InjR "e1" =>
+          match: "e1" with
+            (* Suspend: *) InjL "suspender" =>
+              (* a.d. probably the most complicated line 
+              When waker is called with a value v, a closure calling the continuation with v is put into the run_queue. 
+              suspender can either put waker somewhere that causes it to be called later or just call it directly. *)
+              let: "waker" := (λ: "v", queue_push "q" (λ: <>, "k" "v")) in
+              "suspender" "waker";;
+              next "result" "q"
+          | (* GetContext: *) InjR <> =>
+              "k" "context"
+          end
+        end)
+    | return (λ: <>, next "result" "q")
+    end)%V.
     
-  Definition run : val := (λ: "main",
-    let: "initial_state" := new_fiber_state #() in
+  Definition run : val := (λ: "init" "main",
+    let: "result" := new_scheduler_result #() in
+    let: "initial_context" := new_context "init" in
     let: "q" := queue_create #() in
-    let: "fulfill" := rec: "fulfill" "state" "f" :=
-      deep-try: "f" #() with
-        effect (λ: "request" "k",
-          match: "request" with
-            (* Fork: *) InjL "statef" =>
-              let: "fork_state" := Fst "statef" in
-              let: "fork_f" := Snd "statef" in
-              queue_push "q" (λ: <>, "k" #());;
-              "fulfill" "fork_state" "fork_f"
-          | (* Suspend/GetContext: *) InjR "e1" =>
-            match: "e1" with
-              (* Suspend: *) InjL "suspender" =>
-                (* a.d. probably the most complicated line 
-                When waker is called with a value v, a closure calling the continuation with v is put into the run_queue. 
-                suspender can either put waker somewhere that causes it to be called later or just call it directly. *)
-                let: "waker" := (λ: "v", queue_push "q" (λ: <>, "k" "v")) in
-                "suspender" "waker";;
-                next "q"
-            | (* GetContext: *) InjR <> =>
-                "k" "state"
-            end
-          end)
-      | return (λ: <>, next "q")
-      end
-    in
-    "fulfill" "initial_state" "main"
+    execute "q" "result" "initial_context" (λ: <>, "result" <- SOME ("main" #()));;
+    match: Load "result" with
+      (* Not Done *) InjL <> => #() #() (* unreachable *)
+    | (* Done *) InjR "x" => "x"
+    end
   )%V.
 
 End implementation.
@@ -189,7 +212,8 @@ Class promiseGpreS Σ := {
     (authR (gmapUR (loc * gname * gname) unitR));
   (* state_mapG :> inG Σ
     (authR (gmapUR gname (agreeR locO))); *)
-  torchG :> inG Σ (csumR fracR (agreeR unitO));
+  (* mainG :> inG Σ (csumR fracR (agreeR valO)); *)
+  torchG :> inG Σ (csumR fracR (agreeR valO));
   stateG :> inG Σ (agreeR locO);
 }.
   
@@ -199,7 +223,8 @@ Definition promiseΣ := #[
     (gmapURF (loc * gname * gname) unitR));
   (* GFunctor (authRF
     (gmapURF gname (agreeR locO))); *)
-  GFunctor (csumR fracR (agreeR unitO));
+  (* GFunctor (csumR fracR (agreeR valO)); *)
+  GFunctor (csumR fracR (agreeR valO));
   GFunctor (agreeR locO)
 ].
   
@@ -225,20 +250,31 @@ Section predicates.
      When the fiber is done, it updates the state to done. *)
   Definition promise_state_whole γ := own γ (Cinl 1%Qp).
   Definition promise_state_waiting γ := own γ (Cinl (1/2)%Qp).
-  Definition promise_state_done γ := own γ (Cinr (to_agree ())).
+  Definition promise_state_done γ v := own γ (Cinr (to_agree v)).
   
   (* a.d. TODO I wonder if we can reformulate isMember so that we don't even need isState.
      We need it so that we have a single gname γ to identify each thread for use in the GetContext effect.
      *)
-  Definition isFiberState δ (l: loc): iProp Σ :=
-    own δ (to_agree l).
+  Definition tlvAgree δ (l: loc): iProp Σ :=
+      own δ (to_agree l).
+  
+  Definition isTlvPred δ (I : val -> iProp Σ) :=
+      saved_pred_own δ I.
     
-  Definition fiberState δ (l : loc) : iProp Σ := 
-    (isFiberState δ l ∗ ∃ (n:nat), l ↦ #n)%I.
+  Definition isFiberContext (δ : (gname * gname)) (l : loc) : iProp Σ := 
+    let (δ1, δ2) := δ in
+      tlvAgree δ1 l ∗ (∃ v (I : val -d> iPropO Σ), isTlvPred δ2 I ∗ l ↦ v ∗ I v)%I.
+
+  Definition isMainResult (θ : (gname * gname)) ℓres : iProp Σ := 
+    let (θ1, θ2) := θ in (
+    ∃ (Φ : val -> iProp Σ), saved_pred_own θ2 Φ ∗ (
+    (ℓres ↦ NONE' ∗ promise_state_waiting θ1)
+  ∨ (∃ (v: val), ℓres ↦ SOME' v ∗ promise_state_done θ1 v ∗ □ Φ v))
+  )%I.
 
   (* This resource is always held by the active fiber, so we need to pass it in and out of effects 
      and need it as a precondition of a ready fiber. *)
-  Definition fiberContext δ := (∃ (l : loc), fiberState δ l)%I.
+  Definition fiberResources (δ : ((gname * gname) * (gname * gname))) (ℓres : loc) := ((∃ (l : loc), isFiberContext (fst δ) l) ∗ isMainResult (snd δ) ℓres)%I.
     
   (* Fragment of the promise map. *)
   Definition isMember p γ ε :=
@@ -290,7 +326,7 @@ Section predicates.
     ∃ M, isPromiseMap M ∗
       ([∗ map] args ↦ tt ∈ M, let '(p, γ, ε) := args in
         ((* Fulfilled: *) ∃ y,
-          p ↦ Done' y ∗ promise_state_done γ ∗ 
+          p ↦ Done' y ∗ promise_state_done γ y ∗ 
           ∃ (Φ: val -d> iPropO Σ), isPromiseResult ε Φ ∗ □ Φ y)
       ∨
         ((* Unfulfilled: *) ∃ wakers,
@@ -306,15 +342,23 @@ Section predicates.
   Global Instance promiseInv_Persistent : Persistent promiseInv.
   Proof. by apply _. Qed.
 
+  (* Definition main_whole θ := own θ (Cinl 1%Qp).
+  Definition main_running θ := own θ (Cinl (1/2)%Qp).
+  Definition main_done θ (v: val) := own θ (Cinr (to_agree v)).
+
+  Global Instance main_done_Persistent θ v : Persistent (main_done θ v).
+  Proof. by apply _. Qed. *)
+
   (* Now ready is just a predicate on a continuation k, that k is safe to execute under the assumption
-     that promiseInv holds. *)
-  Definition ready (δ : gname) (k: val) : iProp Σ := (
-    fiberContext δ -∗ promiseInv -∗ EWP (k #()) {{ _, True }}
+     that promiseInv holds.
+    a.d. TODO remove promiseInv *)
+  Definition ready δ ℓres (k: val) : iProp Σ := (
+    fiberResources δ ℓres -∗ EWP (k #()) {{ _, fiberResources δ ℓres ∗ ∃ v, promise_state_done (fst (snd δ)) v }}
   )%I.
 
   Definition promiseSt p γ ε: iProp Σ :=
     ((* Fulfilled: *) ∃ y,
-       p ↦ Done' y ∗ promise_state_done γ ∗
+       p ↦ Done' y ∗ promise_state_done γ y ∗
        ∃ (Φ: val -d> iPropO Σ), isPromiseResult ε Φ ∗ □ Φ y)
   ∨
     ((* Unfulfilled: *) ∃ wakers,
@@ -326,7 +370,7 @@ Section predicates.
       
   Definition promiseSt_later p γ ε : iProp Σ :=
     ((* Fulfilled: *) ∃ y,
-       p ↦ Done' y ∗ promise_state_done γ ∗
+       p ↦ Done' y ∗ promise_state_done γ y ∗
        ∃ (Φ: val -d> iPropO Σ), ▷ (isPromiseResult ε Φ ∗ □ Φ y))
   ∨
     ((* Unfulfilled: *) ∃ wakers,
@@ -365,7 +409,7 @@ Section predicates.
   (* Logical rules governing the predicate [torch]. *)
   Section promise_state.
 
-    Global Instance promise_state_done_Persistent γ : Persistent (promise_state_done γ).
+    Global Instance promise_state_done_Persistent γ v : Persistent (promise_state_done γ v).
     Proof. by apply _. Qed.
 
     Lemma promise_state_create : ⊢ |==> ∃ γ, promise_state_whole γ.
@@ -399,8 +443,8 @@ Section predicates.
       by rewrite Qp_half_half.
     Qed.
 
-    Lemma promise_state_fulfill γ :
-      ⊢ promise_state_whole γ ==∗ promise_state_done γ.
+    Lemma promise_state_fulfill γ v :
+      ⊢ promise_state_whole γ ==∗ promise_state_done γ v.
     Proof.
       iApply own_update.
       apply cmra_update_exclusive.
@@ -408,22 +452,13 @@ Section predicates.
       done.
     Qed.
     
-    Lemma promise_state_disjoint γ : (promise_state_waiting γ ∗ promise_state_done γ) -∗ False.
+    Lemma promise_state_disjoint γ v : (promise_state_waiting γ ∗ promise_state_done γ v) -∗ False.
     Proof. 
       by rewrite /promise_state_waiting /promise_state_done -own_op own_valid csum_validI.
     Qed.
 
-  End promise_state.
-  
-  Section fiber_state.
-    Global Instance isFiberState_persistent δ l: Persistent (isFiberState δ l).
-    Proof. by apply _. Qed.
-
-    Lemma fiber_state_create (l: loc) : ⊢ |==> ∃ δ, isFiberState δ l.
-    Proof. by iMod (own_alloc (to_agree l)) as (δ) "Hfs"; last iExists δ. Qed.
-    
-    Lemma is_fiber_state_agree (l l' : loc) δ : 
-      isFiberState δ l -∗ isFiberState δ l' -∗ ⌜ l = l' ⌝.
+    Lemma promise_state_done_agree γ (v v' : val) : 
+      promise_state_done γ v -∗ promise_state_done γ v' -∗ ⌜ v = v' ⌝.
     Proof.
       iIntros "H H'". 
       iCombine "H H'" as "H".
@@ -432,25 +467,98 @@ Section predicates.
       by apply to_agree_op_inv_L.
     Qed.
 
-    Lemma fiber_state_agree (l l' : loc) δ : 
-      fiberState δ l -∗ isFiberState δ l' -∗ ⌜ l = l' ⌝ ∗ fiberState δ l.
+  End promise_state.
+  
+  Section fiber_state.
+    Global Instance tlvAgree_persistent δ l: Persistent (tlvAgree δ l).
+    Proof. by apply _. Qed.
+
+    Lemma fiber_context_create (l: loc) : ⊢ |==> ∃ δ, tlvAgree δ l.
+    Proof. by iMod (own_alloc (to_agree l)) as (δ) "Hfs"; last iExists δ. Qed.
+
+    Lemma tlvAgree_agree (l l' : loc) δ : 
+      tlvAgree δ l -∗ tlvAgree δ l' -∗ ⌜ l = l' ⌝.
     Proof.
+      iIntros "H H'". 
+      iCombine "H H'" as "H".
+      iPoseProof (own_valid with "H") as "%".
+      iPureIntro.
+      by apply to_agree_op_inv_L.
+    Qed.
+
+    Lemma isFiberContext_agree (l l' : loc) δ : 
+      isFiberContext δ l -∗ tlvAgree (fst δ) l' -∗ ⌜ l = l' ⌝ ∗ isFiberContext δ l.
+    Proof.
+      rewrite /isFiberContext.
+      destruct δ as [δ1 δ2].
       iIntros "(#H & HRest) #H'". 
-      iSplitR; first by iApply is_fiber_state_agree.
+      iSplitR; first by iApply tlvAgree_agree.
       by iFrame.
     Qed.
     
-    Lemma fiber_context_agree (l : loc) δ :
-      fiberContext δ -∗ isFiberState δ l -∗ fiberState δ l.
+    Lemma isFiberContext_tlvAgree l δ :
+      isFiberContext δ l -∗ tlvAgree (fst δ) l ∗ isFiberContext δ l.
     Proof.
-      iIntros "(% & HfState) H".
-      by iDestruct (fiber_state_agree with "HfState H") as (->) "HfState".
+      iIntros "HfCtx".
+      rewrite /isFiberContext.
+      destruct δ as [δ1 δ2].
+      iDestruct "HfCtx" as "[#HtlvAg $]".
+      by iSplit.
     Qed.
   End fiber_state.
 
   (* Logical rules governing the predicate [ready]. *)
   Section ready.
+    (* a.d. TODO remove and unify with promise_state *)
+    (* Lemma main_running_split θ :
+      main_whole θ ==∗ main_running θ ∗ main_running θ.
+    Proof.
+      rewrite /main_running.
+      rewrite -own_op.
+      iApply own_update.
+      rewrite -Cinl_op.
+      apply csum_update_l.
+      rewrite frac_op.
+      rewrite cmra_update_updateP.
+      apply cmra_updateP_id. 
+      apply Qp_half_half.
+    Qed.
 
+    Lemma main_running_join θ :
+      ⊢ main_running θ ∗ main_running θ ==∗ main_whole θ.
+    Proof.
+      rewrite /main_running.
+      rewrite -own_op.
+      iApply own_update.
+      rewrite -Cinl_op.
+      apply csum_update_l.
+      rewrite frac_op.
+      rewrite cmra_update_updateP.
+      apply cmra_updateP_id. 
+      by rewrite Qp_half_half.
+    Qed.
+
+    Lemma isMainResult_alloc result : 
+      result ↦ NONE' ==∗ ∃ θ, isMainResult θ result ∗ main_running θ.
+    Proof.
+      iIntros "Hres".
+      iMod (own_alloc (Cinl (1%Qp))) as (θ) "Hrun"; first by done.
+      iMod (main_running_split with "Hrun") as "[Hrun1 Hrun2]".
+      iModIntro. iExists _.
+      iSplitR "Hrun2".
+      iLeft. by iFrame. 
+      by iAssumption.
+    Qed.
+
+    Lemma main_complete θ v :
+      ⊢ main_whole θ ==∗ main_done θ v.
+    Proof.
+      iIntros "H".
+      iApply (own_update with "H").
+      apply cmra_update_exclusive.
+      apply Cinr_valid.
+      done.
+    Qed. *)
   End ready.
 
   (* Logical rules governing the predicates [isPromiseMap], [isPromise], and
@@ -569,28 +677,26 @@ End predicates.
 Section protocol_coop.
   Context `{!heapGS Σ, !promiseGS Σ, !savedPredG Σ val}.
   
-  Notation pEff := (gnameO -d> iEffO) (only parsing).
-  
-  Definition FORK_pre (Coop : pEff) (δ : gname): iEff Σ :=
-    >> (ℓstate : loc) e >> !(Fork' #ℓstate e) {{fiberState δ ℓstate ∗ ▷ (fiberContext δ -∗ EWP e #() <|Coop δ |> {{_, fiberContext δ}}) }};
-    << (_: val) << ?(#())        {{ fiberState δ ℓstate }} @ OS.
-      (* a.d. TODO I think I can delete promiseInv from SUSPEND *)
+  Notation pEff := (((gnameO * gnameO) * (gnameO * gnameO) * loc) -d> iEffO) (only parsing).
 
-  Definition SUSPEND (δ : gname) : iEff Σ :=
+  Definition FORK_pre (Coop : pEff) (δℓ : ((gname * gname) * (gname * gname) * loc)) : iEff Σ :=
+    >> (ℓtlv : loc) e >> !(Fork' #ℓtlv e) {{fiberResources (fst δℓ) (snd δℓ) ∗ tlvAgree (fst (fst (fst δℓ))) ℓtlv ∗ ▷ (fiberResources (fst δℓ) (snd δℓ) -∗ EWP e #() <|Coop δℓ |> {{_, fiberResources (fst δℓ) (snd δℓ) }}) }};
+    << (_: val) << ?(#())        {{ fiberResources (fst δℓ) (snd δℓ) }} @ OS.
+
+  Definition SUSPEND (δℓ : ((gname * gname) * (gname * gname) * loc)) : iEff Σ :=
     >> (f: val) (P: val → iProp Σ) >> !(Suspend' f) {{
+        fiberResources (fst δℓ) (snd δℓ) ∗
       (* We call suspender with the waker function and waker receives a value satisfying P. *)
-        ( (∀ (waker: val),
+        (∀ (waker: val),
           (∀ (v: val), P v -∗  (EWP (waker v) <| ⊥ |> {{_, True }}) ) -∗
           (▷ EWP (f waker) <| ⊥ |> {{_, True  }}) ) 
-      ∗
-        fiberContext δ)%I
     }};
-    << y           << ?(y)         {{ P y ∗ fiberContext δ }} @ OS.
+    << y           << ?(y)         {{ fiberResources (fst δℓ) (snd δℓ) ∗ P y }} @ OS.
 
-  Definition GET_CONTEXT (δ: gname ): iEff Σ :=
+  Definition GET_CONTEXT (δℓ : ((gname * gname) * (gname * gname) * loc)) : iEff Σ :=
     >> (_: val) >> !(GetContext') {{ True }};
-    << (state : loc) << ?(#state) 
-        {{isFiberState δ state}} @ OS.
+    << (ℓtlv : loc) << ?(#ℓtlv) 
+        {{ tlvAgree (fst (fst (fst δℓ))) ℓtlv }} @ OS.
 
   Definition Coop_pre : pEff → pEff := (λ Coop,
     λ δ, FORK_pre Coop δ <+> SUSPEND δ <+> GET_CONTEXT δ
@@ -602,7 +708,7 @@ Section protocol_coop.
     rewrite /Coop_pre /SUSPEND /FORK_pre /GET_CONTEXT=> n Coop Coop' HCoop.
     by repeat (apply ewp_ne||apply iEffPre_base_ne||f_contractive||f_equiv).
   Qed.
-  Definition Coop_def : (gname → iEff Σ) := fixpoint Coop_pre.
+  Definition Coop_def : (((gname * gname) * (gname * gname) * loc) → iEff Σ) := fixpoint Coop_pre.
   Definition Coop_aux : seal Coop_def. Proof. by eexists. Qed.
   Definition Coop := Coop_aux.(unseal).
   Definition Coop_eq : Coop = Coop_def := Coop_aux.(seal_eq).
@@ -623,32 +729,33 @@ Section protocol_coop.
     - by rewrite upcl_sum upcl_sum (upcl_tele' [tele _ _] [tele _]) //.
   Qed.
 
-  Lemma upcl_FORK δ v Φ' :
-    iEff_car (upcl OS (FORK δ)) v Φ' ≡
-      (∃ (ℓstate: loc) e, ⌜ v = Fork' #ℓstate e ⌝ ∗ (fiberState δ ℓstate ∗ ▷ (fiberContext δ -∗ EWP e #() <|Coop δ|> {{_, fiberContext δ }})) ∗
-            (∀ (_ : val), fiberState δ ℓstate -∗ Φ' #()))%I.
+  Lemma upcl_FORK δℓ v Φ' :
+    iEff_car (upcl OS (FORK δℓ)) v Φ' ≡
+      (∃ (ℓtlv : loc) e, ⌜ v = Fork' #ℓtlv e ⌝ ∗ (fiberResources (fst δℓ) (snd δℓ) ∗ tlvAgree (fst (fst (fst δℓ))) ℓtlv ∗ ▷ (fiberResources (fst δℓ) (snd δℓ) -∗ EWP e #() <|Coop δℓ|> {{_, fiberResources (fst δℓ) (snd δℓ) }})) ∗
+            (∀ (_ : val), fiberResources (fst δℓ) (snd δℓ) -∗ Φ' #()))%I.
   Proof. by rewrite /FORK (upcl_tele' [tele _ _] [tele _]). Qed.
 
   Lemma upcl_SUSPEND δ v Φ' :
     iEff_car (upcl OS (SUSPEND δ)) v Φ' ≡
       (∃ (f : val) (P: val → iProp Σ), ⌜ v = Suspend' f ⌝ 
       ∗ 
-      (* the big precondition of the protocol *)
-        ( (∀ (waker: val),
+      ( fiberResources (fst δ) (snd δ) ∗ 
+        (∀ (waker: val),
           (∀ (v: val), P v -∗ (EWP (waker v) <| ⊥ |> {{_, True }}) ) -∗
-          (▷ EWP (f waker) <| ⊥ |> {{_, True }}) )
+          (▷ EWP (f waker) <| ⊥ |> {{_, True }}) ) )
       ∗
-          fiberContext δ) 
-      ∗
-          (∀ v, (P v ∗ fiberContext δ) -∗ Φ' v))%I.
+          (∀ v, (fiberResources (fst δ) (snd δ) ∗ P v ) -∗ Φ' v))%I.
   Proof. by rewrite /SUSPEND (upcl_tele' [tele _ _] [tele _]). Qed.
 
-  Lemma upcl_GET_CONTEXT δ v Φ' :
+  Lemma upcl_GET_CONTEXT (δ : (gname * gname) * (gname * gname) * loc) v Φ' :
     iEff_car (upcl OS (GET_CONTEXT δ)) v Φ' ≡ 
       (∃ (_: val), ⌜ v = GetContext' ⌝ ∗ True ∗
-        (∀ (ℓstate : loc), isFiberState δ ℓstate -∗ Φ' #ℓstate)
+        (∀ (ℓstate : loc), tlvAgree (fst (fst (fst δ))) ℓstate -∗ Φ' #ℓstate)
       )%I.
-  Proof. by rewrite /GET_CONTEXT (upcl_tele' [tele _] [tele _]). Qed.
+  Proof.
+    destruct δ as [δ1 δ2].
+    by rewrite /GET_CONTEXT (upcl_tele' [tele _] [tele _]). 
+  Qed.
 
 End protocol_coop.
 
@@ -657,14 +764,36 @@ End protocol_coop.
 (** * Verification. *)
 
 Section verification.
-  Context `{!heapGS Σ, !promiseGS Σ, !ListLib Σ, !savedPredG Σ val}.
+  Context `{!heapGS Σ, !promiseGS Σ, !savedPredG Σ val}.
+
+  Lemma ewp_new_scheduler_result (Φ : val -> iProp Σ) :
+    ⊢ EWP (new_scheduler_result #()) {{ v, ∃ θ (ℓres : loc), ⌜ v = #ℓres ⌝ ∗ isMainResult θ ℓres ∗ promise_state_waiting (fst θ) ∗ saved_pred_own (snd θ) Φ }}.
+  Proof.
+    rewrite /new_scheduler_result.
+    ewp_pure_steps.
+    iApply ewp_alloc.
+    iIntros "!> %ℓres Hres".
+    iMod promise_state_create as (θ1) "Hwhole".
+    iMod (promise_state_split with "Hwhole") as "[Hrun1 Hrun2]".
+    iMod (saved_pred_alloc Φ) as "[%θ2 #Hθ2]".
+    iModIntro.
+    iExists (θ1, θ2), _. iSplit; first done.
+    iSplitL "Hres Hrun1".
+    rewrite /isMainResult.
+    iExists _. iSplit; first by done.
+    iLeft. by iFrame.
+    by iSplit.
+  Qed.
 
   Lemma ewp_new_promise Φ :
     promiseInv ⊢ EWP (new_promise #()) {{ y,
         ∃ p γ ε, ⌜ y = #(p : loc) ⌝ ∗ promise_state_waiting γ ∗ isMember p γ ε ∗ isPromiseResult ε Φ}}.
   Proof.
     iIntros "HpInv".
-    unfold new_promise. ewp_pure_steps. ewp_bind_rule. simpl.
+    unfold new_promise. ewp_pure_steps. 
+    (* a.d. TODO here it should be okay to use ewp_bind_rule. Something is broken. *)
+    iApply (ewp_bind' (AllocNRCtx _)); first by done. simpl.
+    iApply (ewp_bind' (InjRCtx)); first by done. simpl.
     iApply ewp_mono. { by iApply newThreadQueue_spec. }
     iIntros (enqs) "(#Hcqs & Htqstate & Hres) !>". ewp_pure_steps.
     (* open the invariant -> evaluate the alloc -> change and close the invariant *)
@@ -690,62 +819,106 @@ Section verification.
     iExists p, γ, ε. iFrame. by auto.
   Qed.
   
-  Lemma ewp_new_fiber_state :
-    ⊢ EWP new_fiber_state #() {{ state, ∃ (ℓstate : loc) (n: nat), ⌜ state = #ℓstate ⌝ ∗ ℓstate ↦ #n }}.
+  Lemma ewp_new_context init (I : val -> iProp Σ) :
+    I init ⊢ EWP new_context init {{ tlv, ∃ (ℓtlv : loc) δ, ⌜ tlv = #ℓtlv ⌝ ∗ isFiberContext δ ℓtlv }}.
   Proof.
-    iIntros. rewrite /new_fiber_state.
-    ewp_pure_steps. iApply ewp_alloc.
-    iIntros "!>" (ℓstate) "Hstate !>".
-    iExists _, 0. by iFrame. 
+    iIntros "HI". rewrite /new_context.
+    ewp_pure_steps.
+    iMod (saved_pred_alloc I) as "[%δ2 #Hδ1]".
+    iApply ewp_alloc.
+    iIntros "!>" (ℓtlv) "Htlv".
+    iMod (fiber_context_create ℓtlv) as "[%δ1 #HtlvAg]".
+    iModIntro.
+    iExists ℓtlv, (δ1, δ2).
+    iSplit; first by done.
+    iSplit; first by done.
+    iExists init, I.
+    by iFrame.
   Qed.
     
-  Lemma ewp_next δ q Ψ :
-    fiberContext δ -∗
-    promiseInv -∗
-      is_queue q (ready δ) -∗
-         EWP (next q) <| Ψ |> {{ _, True }}.
+  Lemma ewp_next δ ℓres q Ψ :
+    fiberResources δ ℓres ∗ is_queue q (ready δ ℓres) 
+  ⊢
+    EWP (next #ℓres q) <| Ψ |> {{ _, fiberResources δ ℓres ∗ ∃ v, promise_state_done (fst (snd δ)) v }}.
   Proof.
-    iIntros "HfCtx HpInv #Hq". unfold next. ewp_pure_steps. ewp_bind_rule.
+    iLöb as "IH".
+    iIntros "(HfRes & #Hq)". unfold next. ewp_pure_steps. ewp_bind_rule.
     iApply ewp_mono; [iApply (queue_pop_spec with "Hq")|].
-    simpl. iIntros (y) "[->|(%k & -> & Hk)] !>".
+    destruct δ as ((δ11 & δ12) & (δ21 & δ22)).
+    simpl.
+    iIntros (y) "[->|(%k & -> & Hk)] !>".
     - (* queue is empty *) 
-      by ewp_pure_steps.
+      ewp_pure_steps.
+      ewp_bind_rule; simpl.
+      iDestruct "HfRes" as "[HfRes Hres]".
+      iDestruct "Hres" as "(% & #Hsaved & [(Hres&HRest)|(%&Hres&#Hdone&#HΦ)])".
+      + (* Main fiber is not done. Busy wait. *)
+        iApply (ewp_load with "Hres").
+        iIntros "!> Hres !>".
+        do 4 ewp_value_or_step. 
+        iApply "IH". iFrame. iSplit; last done.
+        iExists _. iSplit; first done. 
+        iLeft. by iFrame.
+      + (* Main fiber is done. *)
+        iApply (ewp_load with "Hres").
+        iIntros "!> Hres !>".
+        ewp_pure_steps. 
+        iSplitL "HfRes Hres".
+        iFrame. 
+        iExists _. iSplit; first by done. 
+        iRight. iExists _. iFrame. by iSplit.
+        by iExists _.
     - (* queue has a continuation *)
       ewp_pure_steps.
-      rewrite /ready.
-      iSpecialize ("Hk" with "HfCtx HpInv").
+      rewrite {3}/ready.
+      iSpecialize ("Hk" with "HfRes").
       iApply ewp_os_prot_mono. { by iApply iEff_le_bottom. } { done. }
   Qed.
 
-  Lemma ewp_fork (ℓstate : loc) (e : val) δ :
-    fiberState δ ℓstate ∗ (fiberContext δ -∗ EWP e #() <| Coop δ|> {{ _, fiberContext δ }})
+  Lemma ewp_fork (ℓstate ℓres: loc) (e : val) δ :
+    fiberResources δ ℓres ∗ tlvAgree (fst (fst δ)) ℓstate ∗ (fiberResources δ ℓres -∗ EWP e #() <| Coop (δ, ℓres) |> {{ _, fiberResources δ ℓres }})
   ⊢
-      EWP (fork #ℓstate e) <| Coop δ |> {{ _, fiberState δ ℓstate }}.
+    EWP (fork #ℓstate e) <| Coop (δ, ℓres) |> {{ _, fiberResources δ ℓres }}.
   Proof.
-    iIntros "(Hfstate & He)". rewrite /fork. ewp_pure_steps.
+    iIntros "(HfRes & HtlvAg & He)". rewrite /fork. ewp_pure_steps.
     iApply ewp_do_os. rewrite upcl_Coop upcl_FORK. iLeft.
-    iExists ℓstate, e. iSplit; [done|]. iFrame.
+    iExists ℓstate, e. iSplit; first by done. iFrame.
     iIntros (_) "H". by done.
   Qed.
 
-  Lemma ewp_suspend (f : val) (P: val → iProp Σ) δ :
-      ( (∀ (waker: val),
+  Lemma ewp_suspend (ℓres : loc) (f : val) (P: val → iProp Σ) δ :
+    ( fiberResources δ ℓres ∗
+      (∀ (waker: val),
         (∀ (v: val), P v -∗ (EWP (waker v) <| ⊥ |> {{_, True}}) ) -∗
-        (▷ EWP (f waker) <| ⊥ |> {{_, True }})) 
-    ∗
-      fiberContext δ) 
+        (▷ EWP (f waker) <| ⊥ |> {{_, True }})) ) 
     ⊢
-      EWP (suspend f) <| Coop δ |> {{ v, P v ∗ fiberContext δ }}.
+      EWP (suspend f) <| Coop (δ, ℓres) |> {{ v, fiberResources δ ℓres ∗ P v }}.
   Proof.
-    iIntros "(He & HpInv)". rewrite /suspend. ewp_pure_steps.
+    iIntros "(HfRes & He)". rewrite /suspend. ewp_pure_steps.
     iApply ewp_do_os. rewrite upcl_Coop upcl_SUSPEND. iRight; iLeft.
     iExists f, P. iSplit; [done|]. iFrame.
     iIntros (v) "Hv". by iFrame.
   Qed.
-  
-  Lemma ewp_get_context δ : 
-    ⊢ EWP (get_context #()) <| Coop δ |> {{ state, ∃ (ℓstate: loc), ⌜ state = #ℓstate ⌝ ∗ isFiberState δ ℓstate }}.
+
+  Lemma ewp_yield (ℓres : loc) δ :
+    fiberResources δ ℓres
+  ⊢ 
+    EWP (yield #()) <| Coop (δ, ℓres) |> {{ _, fiberResources δ ℓres }}.
   Proof.
+    iIntros "HfRes".
+    rewrite /yield. ewp_pure_steps.
+    iApply (ewp_mono with "[HfRes]"); first iApply (ewp_suspend _ _ (λ _, True)%I).
+    { iFrame. iIntros (waker) "Hwaker". 
+      iSpecialize ("Hwaker" $! #() with "[$]").
+      iNext. ewp_pure_steps. iApply "Hwaker". }
+    iIntros (?) "[$ _] !>".
+    done.
+  Qed.
+  
+  Lemma ewp_get_context ℓres δ : 
+    ⊢ EWP (get_context #()) <| Coop (δ, ℓres) |> {{ tlv, ∃ (ℓtlv: loc), ⌜ tlv = #ℓtlv ⌝ ∗ tlvAgree (fst (fst δ)) ℓtlv }}.
+  Proof.
+    destruct δ as [δ1 δ2] eqn:E.
     iIntros. rewrite /get_context. ewp_pure_steps.
     iApply ewp_do_os. rewrite upcl_Coop upcl_GET_CONTEXT. iRight; iRight.
     iExists #(). iSplit; [done|]. iSplit; [done|].
@@ -757,7 +930,7 @@ Section verification.
     promiseInv ∗ suspension_permit ∗ isMember p γ ε ∗ isPromiseResult ε Φ ∗ promise_cqs wakers 
   ⊢
     EWP (await_callback #p wakers) <| ⊥ |> {{f, 
-      ∀ (waker: val), (∀ (v: val), (⌜ v = #() ⌝ ∗ promise_state_done γ)%I -∗ EWP (waker v) <| ⊥ |> {{_, True }}) -∗
+      ∀ (waker: val), (∀ (v: val), (⌜ v = #() ⌝ ∗ ∃ v', promise_state_done γ v')%I -∗ EWP (waker v) <| ⊥ |> {{_, True }}) -∗
         (▷ EWP (f waker) <| ⊥ |> {{_, True }}) }}.
   Proof.
     iIntros "(#HpInv & HIsSus & #Hmem & #Hε & #Hcqs)". rewrite /await_callback. ewp_pure_steps.
@@ -766,7 +939,7 @@ Section verification.
     (* now we suspend waker*)
     iApply (ewp_bind' (AppRCtx _)); first by done. simpl.
     iApply (ewp_mono with "[HIsSus Hwaker]").
-    { iApply (cqs_suspend_spec (promise_state_done γ) with "[HIsSus Hwaker]").
+    { iApply (cqs_suspend_spec (∃ v', promise_state_done γ v') with "[HIsSus Hwaker]").
       iFrame.
       by done.
     }
@@ -795,7 +968,7 @@ Section verification.
       ewp_pure_steps.
       iApply (ewp_bind' (IfCtx _ _)); first by done. simpl.
       iApply (ewp_mono with "[Hreq]").
-      iApply (cqs_try_cancel_spec (promise_state_done γ) with "[Hreq]").
+      iApply (cqs_try_cancel_spec (∃ v', promise_state_done γ v') with "[Hreq]").
       by iFrame.
       iIntros (?) "(% & -> & Hk) !>".
       destruct b.
@@ -804,7 +977,10 @@ Section verification.
         ewp_pure_steps. by done.
       }
       ewp_pure_steps.
-      iApply "Hk". by iSplit.
+      iApply "Hk".
+      rewrite /V'.
+      iSplit; first done.
+      iExists _. by iAssumption.
     - (* the promise is not yet fulifilled, our job is done and we don't do anything *)
       iApply (ewp_load with "Hp").
       iIntros "!> Hp !>". 
@@ -817,9 +993,9 @@ Section verification.
       + ewp_pure_steps. by done.
   Qed.
   
-  Lemma ewp_await (p: loc) Φ δ :
-    fiberContext δ ∗ promiseInv ∗ isPromise p Φ ⊢ 
-      EWP (await #p) <| Coop δ |> {{v, □ Φ v ∗ fiberContext δ}}.
+  Lemma ewp_await (ℓres p: loc) Φ δ :
+    fiberResources δ ℓres ∗ promiseInv ∗ isPromise p Φ ⊢ 
+      EWP (await #p) <| Coop (δ, ℓres) |> {{v, □ Φ v ∗ fiberResources δ ℓres }}.
   Proof.
     iIntros "(HfCtx & #HpInv & %γ & %ε & #Hmem & #Hε)". rewrite /await. 
     ewp_pure_steps. ewp_bind_rule. simpl.
@@ -869,10 +1045,10 @@ Section verification.
       ewp_pure_steps.
       ewp_bind_rule. simpl.
       iApply (ewp_mono with "[Hf HfCtx]").
-      { iApply (ewp_suspend callback (λ v, ⌜ v = #() ⌝ ∗ promise_state_done γ)%I). 
+      { iApply (ewp_suspend _ callback (λ v, ⌜ v = #() ⌝ ∗ ∃ v', promise_state_done γ v')%I). 
         by iFrame. }
       (* after we have performed the effect we get promise_state_done. *)
-      iIntros (v) "((-> & Hps) & HfCtx) !>".
+      iIntros (v) "(HfCtx & (-> & (%&Hps))) !>".
       ewp_pure_steps. ewp_bind_rule. simpl.
       (* now we match on the promise again but this time we know it must be fulfilled *)
       iClear "Hwakers". clear wakers.
@@ -880,7 +1056,8 @@ Section verification.
       iMod (inv_acc with "HpInv") as "(HpInvIn & Hclose)"; first by done.
       iMod (lookup_promiseInv_inner with "HpInvIn Hmem") as "[HpInvIn HpSt]".
       iDestruct "HpSt" as "[[%y (Hp&#Hps'&%Φ'&#Hε'&#Hy)]| (%wakers & Hp & Hps' & Htqstate & Hres & #Hwakers) ]";
-        last by iDestruct (promise_state_disjoint γ with "[$]") as "HFalse".
+        last by iDestruct (promise_state_disjoint γ _ with "[$]") as "HFalse".
+      iDestruct (promise_state_done_agree with "Hps Hps'") as "->".
       iModIntro.
       iApply (ewp_load with "Hp").
       iIntros "!> Hp !>". 
@@ -889,7 +1066,9 @@ Section verification.
       iSplitL "Hclose". iApply "Hclose".
       iModIntro.
       iSplitR "HfCtx".
-      iNext. iApply "HpInvIn". iLeft. iExists y. iFrame. 
+      iNext. iApply "HpInvIn". iLeft.
+      iExists y. iFrame. 
+      iSplit; first done.
       iExists Φ'. by iSplit.
       ewp_pure_steps.
       iFrame.
@@ -899,13 +1078,13 @@ Section verification.
   (* the wrapped function is passed via the FORK effect to the handler.
      the handler should then pass is_queue to wrapped_f so that it is able to change the run_queue.
      is_queue should be passed between client and handler the same as promiseInv, for every performed effect. *)
-  Lemma ewp_fork_wrap (f: val) (p: loc) γ δ ε Φ :
-    promise_state_waiting γ ∗ isMember p γ ε ∗ isPromiseResult ε Φ ∗ (fiberContext δ -∗ EWP (f #()) <| Coop δ |> {{v, □ Φ v ∗ fiberContext δ}}) 
+  Lemma ewp_fork_wrap (ℓres: loc) (f: val) (p: loc) γ δ ε Φ :
+    promise_state_waiting γ ∗ isMember p γ ε ∗ isPromiseResult ε Φ ∗ (fiberResources δ ℓres -∗ EWP (f #()) <| Coop (δ, ℓres) |> {{v, □ Φ v ∗ fiberResources δ ℓres }}) 
   ⊢
     EWP (fork_wrap_f f #p) <| ⊥ |> {{wrapped_f, 
         (* promiseInv and is_queue are passed here because they come from the effect handler *)
           promiseInv -∗
-          fiberContext δ -∗ EWP (wrapped_f #()) <| Coop δ |> {{_, fiberContext δ }} }}.
+          fiberResources δ ℓres -∗ EWP (wrapped_f #()) <| Coop (δ, ℓres) |> {{_, fiberResources δ ℓres }} }}.
   Proof.
     iIntros "(Hps_start & #Hmem & #Hε & Hf)". 
     rewrite /fork_wrap_f. ewp_pure_steps.
@@ -951,23 +1130,23 @@ Section verification.
     iApply (ewp_mono with "[Htqstate Hres]"). 
     { iApply ewp_os_prot_mono. iApply iEff_le_bottom.
       iDestruct "Htqstate" as (n) "Htqstate".
-      iApply (cqs_resume_all_spec (promise_state_done γ) with "[Htqstate Hres Hwakers]").
+      iApply (cqs_resume_all_spec (∃ v', promise_state_done γ v') with "[Htqstate Hres Hwakers]").
       iFrame. iSplit; first done. 
-      by done. }
+      iModIntro. iNext. by iExists _. }
     iIntros (?) "_ !>". by done.
   Qed.
 
-  Lemma ewp_fork_promise (f: val) Φ δ :
-    fiberContext δ ∗ promiseInv ∗ (fiberContext δ -∗ EWP (f #()) <| Coop δ |> {{v, □ Φ v ∗ fiberContext δ}})
+  Lemma ewp_fork_promise (ℓres : loc) (f: val) Φ δ :
+    fiberResources δ ℓres ∗ promiseInv ∗ (fiberResources δ ℓres -∗ EWP (f #()) <| Coop (δ, ℓres) |> {{v, □ Φ v ∗ fiberResources δ ℓres }})
   ⊢ 
-    EWP (fork_promise f) <| Coop δ |> {{ y, 
-      ∃ (p: loc), ⌜ y = #p ⌝ ∗ isPromise p Φ ∗ fiberContext δ }}.
+    EWP (fork_promise f) <| Coop (δ, ℓres) |> {{ y, 
+      ∃ (p: loc), ⌜ y = #p ⌝ ∗ isPromise p Φ ∗ fiberResources δ ℓres }}.
   Proof.
-    iIntros "(HfCtx & #HpInv & Hf)". rewrite /fork_promise. ewp_pure_steps.
+    iIntros "(HfRes & #HpInv & Hf)". rewrite /fork_promise. ewp_pure_steps.
     ewp_bind_rule. simpl.
     iApply ewp_mono.
     iApply ewp_get_context.
-    iIntros (state) "(%ℓstate & -> & #HIsState) !>".
+    iIntros (tlv) "(%ℓtlv & -> & #HtlvAg) !>".
     ewp_pure_steps.
     ewp_bind_rule. simpl.
     iApply ewp_mono. 
@@ -984,76 +1163,67 @@ Section verification.
     iSpecialize ("Hwrapped_f" with "HpInv").
     ewp_pure_steps.
     iApply (ewp_bind' (AppRCtx _)); first done. simpl.
-    iApply (ewp_mono with "[Hwrapped_f HfCtx]").
+    iApply (ewp_mono with "[Hwrapped_f HfRes]").
     iApply ewp_fork. 
-    iPoseProof (fiber_context_agree with "HfCtx HIsState") as "HfState".
     by iFrame.
     iIntros (?) "HfState !>".
     ewp_pure_steps. iExists p.
     iFrame. iSplit; first done.
-    iSplitR.
     iExists γ, ε. by iSplit.
-    by iExists _.
   Qed.
-      
-  Lemma ewp_run (main : val) Φ :
-    promiseInv ∗ (∀ δ, fiberContext δ -∗ EWP main #() <| Coop δ |> {{ v, □ Φ v ∗ fiberContext δ }}) ⊢
-      EWP run main {{ _, True }}.
+
+  Lemma ewp_execute (q fiber : val) δ ℓres ℓtlv :
+    is_queue q (ready δ ℓres) -∗
+    fiberResources δ ℓres -∗
+    tlvAgree (fst (fst δ)) ℓtlv -∗
+    (fiberResources δ ℓres -∗ EWP fiber #() <| Coop (δ, ℓres) |> {{ _, fiberResources δ ℓres }}) -∗
+      EWP execute q #ℓres #ℓtlv fiber {{_, fiberResources δ ℓres ∗ ∃ v, promise_state_done (fst (snd δ)) v }}.
   Proof.
-    iIntros "(#HpInv & Hmain)". unfold run. ewp_pure_steps.
-    ewp_bind_rule. simpl. iApply ewp_mono. { by iApply ewp_new_fiber_state. }
-    iIntros (state) "H".
-    iDestruct "H" as (ℓstate n) "(-> & Hℓstate)".
-    iMod (fiber_state_create ℓstate) as (δ) "#HIsState".
-    (* a.d. We must do this up here so that ∀ δ does not appear in IH.
-       a.d. TODO can we speciaize Hℓstate, too? *)
-    iSpecialize ("Hmain" $! δ).
-    iModIntro. ewp_pure_steps.
-    ewp_bind_rule. simpl. iApply ewp_mono. { by iApply queue_create_spec. }
-    iIntros (q) "Hq !>". 
-    (* a.d. it's kind of interesting that ready is now also scheduler specific. But it's nice to know that
-       we cannot schedule a fiber in a different scheduler. *)
-    iSpecialize ("Hq" $! (ready δ)).
+    iIntros "Hq HfRes #HtlvAg Hfiber".
+    rewrite /execute.
+    do 6 ewp_value_or_step.
+    iLöb as "IH" forall (fiber).
+    iSpecialize ("Hfiber" with "HfRes").
     ewp_pure_steps.
-    iLöb as "IH" forall (main q Φ n).
-    iSpecialize ("Hmain" with "[Hℓstate]").
-    { rewrite /fiberContext /fiberState. iExists _. iSplit; first done. by iExists _. }
-    iApply (ewp_deep_try_with with "Hmain").
-    iLöb as "IH_handler" forall (q Φ).
+    iApply (ewp_deep_try_with with "Hfiber").
+    iLöb as "IH_handler".
     iDestruct "Hq" as "#Hq".
     rewrite deep_handler_unfold.
     iSplit; [|iSplit]; last (by iIntros (??) "HFalse"; rewrite upcl_bottom).
     (* Return branch. *)
-    - iIntros (?) "(_ & HfCtx)".
+    - iIntros (?) "HfRes".
       ewp_pure_steps. 
-      by iApply (ewp_next with "HfCtx HpInv Hq").
+      iApply ewp_next. iFrame. by iAssumption.
     (* Effect branch. *)
     - iIntros (request k). rewrite upcl_Coop upcl_FORK upcl_SUSPEND upcl_GET_CONTEXT.
-      iIntros "[(%ℓstate' & %e & -> & (HfState' & He) & Hk)
-               |[(%suspender & %P & -> & (Hsuspender & HfCtx) & Hk)
+      iIntros "[(%ℓtlv' & %e & -> & (HfRes'' & #HtlvAg' & He) & Hk)
+               |[(%suspender & %P & -> & (HfCtx & Hsuspender) & Hk)
                |(%_ & -> & _ & Hk)]]".
       (* Fork. *)
-      + iDestruct (fiber_state_agree with "HfState' HIsState") as (->) "HfState'".
+      + iDestruct "HfRes''" as "[HfRes'' Hres]".
+        iDestruct "HfRes''" as (ℓtlv'') "HfCtx''".
+        iDestruct (isFiberContext_agree with "HfCtx'' HtlvAg") as (->) "HfCtx".
+        iDestruct (isFiberContext_agree with "HfCtx HtlvAg'") as (->) "HfCtx".
         ewp_pure_steps.
         iApply (ewp_bind' (AppRCtx _)); first by done. simpl.
         iApply (ewp_mono with "[Hk]").
         { iApply (queue_push_spec with "Hq"). rewrite /ready.
-          iIntros "HfCtx #HpInv'". ewp_pure_steps.
-          iDestruct (fiber_context_agree with "HfCtx HIsState") as "HfState''".
-          iSpecialize ("Hk" $! #() with "HfState''").
+          iIntros "HfRes". ewp_pure_steps.
+          iSpecialize ("Hk" $! #() with "HfRes").
+          (* iApply (ewp_mono _ _ (λ _, isMainResult θ ℓres ∗ (∃ v : valO, promise_state_done θ v ∗ □ Φ v))%I (λ _, isMainResult θ ℓres ∗ (∃ v : valO, promise_state_done θ v))%I with "[Hk Hres]").
+          2: {
+            iIntros (?) "($ & (% & Hdone & _)) !>".
+            by iExists _.
+          } *)
           iApply "Hk". iNext. 
-          by iApply ("IH_handler" with "Hq").
+          iSpecialize ("IH_handler" with "Hq").
+          rewrite -deep_handler_unfold.
+          iApply "IH_handler".
         }
-        iIntros (?) "_ !>". ewp_pure_steps.
-        (* find out the current state. a.d. TODO it should be sufficient to just have n existentially quantified
-           in the precondition of IH. *)
-        iDestruct "HfState'" as "(_ & (% & Hℓstate))".
-        iApply ("IH" with "[He] Hℓstate Hq").
-        { instantiate (1:=(λ _, True)%I).
-          iIntros "HfCtx".
-          iSpecialize ("He" with "HfCtx").
-          iApply (ewp_mono with "He"). 
-          iIntros (?) "HfCtx !>". by iFrame. }
+        iIntros (?) "_ !>". do 3 ewp_value_or_step.
+        iApply ("IH" with "Hq [Hres HfCtx] He").
+        iFrame.
+        by iExists _.
       (* Suspend/GetContext. *)
       + do 12 ewp_value_or_step.
         ewp_bind_rule. simpl.
@@ -1067,10 +1237,12 @@ Section verification.
           iIntros (v) "HP".
           ewp_pure_steps.
           iApply (queue_push_spec with "Hq"). rewrite /ready.
-          iIntros "HfCtx _". ewp_pure_steps.
+          iIntros "HfRes". ewp_pure_steps.
           iSpecialize ("Hk" $! v with "[$]").
           iApply "Hk". iNext.
-          by iApply ("IH_handler" with "Hq").
+          iSpecialize ("IH_handler" with "Hq").
+          rewrite -deep_handler_unfold.
+          iApply "IH_handler".
         }
         iIntros (waker) "Hwaker !>".
         iSpecialize ("Hsuspender" $! waker with "Hwaker").
@@ -1078,12 +1250,80 @@ Section verification.
         ewp_bind_rule. simpl.
         iApply (ewp_mono with "Hsuspender").
         iIntros (?) "_ !>". ewp_pure_steps.
-        iApply (ewp_next with "HfCtx HpInv Hq").
+        iApply (ewp_next).
+        by iFrame.
       + do 12 ewp_value_or_step.
-        iApply ("Hk" with "[$]"). iNext.
-        iApply ("IH_handler" with "Hq").
+        iApply ("Hk" with "HtlvAg"). iNext.
+        iSpecialize ("IH_handler" with "Hq").
+        rewrite -deep_handler_unfold.
+        iApply "IH_handler".
   Qed.
-
+    
+  Lemma ewp_run (init main : val) I Φ :
+    promiseInv ∗ I init ∗ (∀ δ ℓres, fiberResources δ ℓres -∗ EWP main #() <| Coop (δ, ℓres) |> {{ v, □ Φ v ∗ fiberResources δ ℓres }}) ⊢
+      EWP run init main {{ v, □ Φ v }}.
+  Proof.
+    iIntros "(#HpInv & HI & Hmain)". unfold run. ewp_pure_steps.
+    (* Main fiber result *)
+    ewp_bind_rule; simpl. iApply ewp_mono.
+    by iApply (ewp_new_scheduler_result Φ).
+    iIntros (vres) "(%θ & %ℓres & -> & Hres & Hwaiting & #Hsaved) !>".
+    ewp_pure_steps.
+    (* Initial fiber context. *) 
+    ewp_bind_rule. simpl. iApply (ewp_mono with "[HI]"). 
+    { by iApply ewp_new_context. }
+    iIntros (tlv) "(%ℓtlv & %δ & -> & HfCtx) !>".
+    iPoseProof (isFiberContext_tlvAgree with "HfCtx") as "(#HtlvAg & HfCtx)".
+    (* a.d. We must do this up here so that ∀ δ does not appear in IH.
+       a.d. TODO can we speciaize Hℓstate, too? *)
+    iSpecialize ("Hmain" $! (δ, θ) ℓres).
+    ewp_pure_steps.
+    ewp_bind_rule. simpl. iApply ewp_mono. { by iApply queue_create_spec. }
+    iIntros (q) "#Hq !>". 
+    (* a.d. it's kind of interesting that ready is now also scheduler specific. But it's nice to know that
+       we cannot schedule a fiber in a different scheduler. *)
+    iSpecialize ("Hq" $! (ready (δ, θ) ℓres)).
+    ewp_pure_steps.
+    iApply (ewp_bind' (AppRCtx _)); first by done. simpl.
+    iApply (ewp_mono with "[Hmain Hres Hwaiting HfCtx]").
+    { iApply (ewp_execute with "Hq [HfCtx Hres] HtlvAg [Hmain Hwaiting]").
+      { iFrame. by iExists _. }
+      iIntros "HfRes".
+      ewp_pure_steps.
+      iSpecialize ("Hmain" with "HfRes").
+      ewp_bind_rule; simpl. iApply (ewp_mono with "Hmain").
+      iIntros (vres) "(Hv & [HfCtx Hres]) !>".
+      ewp_pure_steps.
+      destruct θ as (θ1 & θ2). simpl.
+      iDestruct "Hres" as "(% & #Hsaved' & [(Hres & HRest)|(% & Hres & Hdone & #HΦ)])";
+        last by iDestruct (promise_state_disjoint with "[$]") as "[]".
+      iApply (ewp_store with "Hres").
+      (* update main_running to main_done *)
+      iIntros "!> Hres".
+      iMod (promise_state_join with "[$]") as "HRest".
+      iMod (promise_state_fulfill _ vres with "HRest") as "#HRest".
+      iModIntro.
+      iFrame.
+      iExists Φ. iSplit; first by done.
+      iRight. iExists _. iFrame. by iAssumption. }
+    - iIntros (?) "(HfRes & (%v' & Hdone)) !>".
+      ewp_pure_steps.
+      iDestruct "HfRes" as "[HfCtx Hres]".
+      simpl.
+      destruct θ as (θ1, θ2).
+      rewrite /isMainResult.
+      iDestruct "Hres" as "(% & #Hsaved' & [(_ & Hwaiting)|(% & Hres & Hdone' & HΦ)])";
+        first by iDestruct (promise_state_disjoint with "[$]") as "[]".
+      iDestruct (promise_state_done_agree with "Hdone' Hdone") as "->".
+      ewp_bind_rule; simpl.
+      iApply (ewp_load with "Hres").
+      iIntros "!> Hres".
+      iDestruct (saved_pred_agree _ _ _ v' with "Hsaved Hsaved'") as "Heq".
+      iModIntro.
+      ewp_pure_steps.
+      iRewrite "Heq".
+      by iAssumption.
+  Qed.
 End verification.
 
 (* ========================================================================== *)
@@ -1091,35 +1331,37 @@ End verification.
 
 Section specification.
   Context `{!heapGS Σ}.
-  Context `{!ListLib Σ}.
 
   Class AsyncCompLib := {
-    coop : gname → iEff Σ;
-    is_fiber_state : gname → loc → iProp Σ;
-    fiber_context : gname → iProp Σ;
+    coop : ((gname * gname) * (gname * gname) * loc) → iEff Σ;
+    tlv_agree : gname → loc → iProp Σ;
+    tlv_agree_Persistent δ ℓtlv : Persistent (tlv_agree δ ℓtlv);
+    fiber_resources : ((gname * gname) * (gname * gname)) → loc → iProp Σ;
     is_promise : val → (val -> iProp Σ) → iProp Σ;
     is_promise_Persistent p Φ : Persistent (is_promise p Φ);
     promise_inv : iProp Σ;
-    fork_spec δ (f : val) Φ :
-      fiber_context δ ∗ promise_inv ∗ (fiber_context δ -∗ EWP f #() <| coop δ |> {{ y, □ Φ y ∗ fiber_context δ }}) -∗
-        EWP fork_promise f <| coop δ |> {{ p, is_promise p Φ ∗ fiber_context δ }};
-    await_spec δ p Φ :
-      fiber_context δ ∗ promise_inv ∗ is_promise p Φ -∗
-        EWP await p <| coop δ |> {{ y, □ Φ y ∗ fiber_context δ }};
-    get_context_spec δ :
-      ⊢ EWP get_context #() <| coop δ |> {{ state, ∃ (ℓstate: loc), ⌜ state = #ℓstate ⌝ ∗ is_fiber_state δ ℓstate }} ;    
+    promise_inv_Persistent : Persistent (promise_inv);
+    fork_spec (ℓres : loc) (δ : (gname * gname) * (gname * gname)) (f : val) Φ :
+      fiber_resources δ ℓres ∗ promise_inv ∗ (fiber_resources δ ℓres -∗ EWP f #() <| coop (δ, ℓres) |> {{ y, □ Φ y ∗ fiber_resources δ ℓres }}) -∗
+        EWP fork_promise f <| coop (δ, ℓres) |> {{ p, is_promise p Φ ∗ fiber_resources δ ℓres }};
+    await_spec ℓres δ p Φ :
+      fiber_resources δ ℓres ∗ promise_inv ∗ is_promise p Φ -∗
+        EWP await p <| coop (δ, ℓres) |> {{ y, □ Φ y ∗ fiber_resources δ ℓres }};
+    get_context_spec ℓres δ :
+      ⊢ EWP get_context #() <| coop (δ, ℓres) |> {{ tlv, ∃ (ℓtlv: loc), ⌜ tlv = #ℓtlv ⌝ ∗ tlv_agree (fst (fst δ)) ℓtlv }} ;    
+    yield_spec ℓres δ :
+      fiber_resources δ ℓres -∗ EWP yield #() <| coop (δ, ℓres) |> {{ _, fiber_resources δ ℓres }} ;
   }.
 
-  Definition run_spec (main : val) :=
-    (* a.d. TODO remove the □ True *)
-    (∀ _ : AsyncCompLib, ∀ δ, fiber_context δ -∗ EWP main #() <| coop δ |> {{ _, □ True ∗ fiber_context δ }}) ={⊤}=∗
-      EWP run main <| ⊥ |> {{ _, True }}.
+  Definition run_spec (init main : val) (I Φ : val -> iProp Σ)  :=
+    I init -∗ 
+    (∀ _ : AsyncCompLib, ∀ δ ℓres, fiber_resources δ ℓres -∗ EWP main #() <| coop (δ, ℓres) |> {{ v, □ Φ v ∗ fiber_resources δ ℓres }}) ={⊤}=∗
+      EWP run init main <| ⊥ |> {{ v, □ Φ v }}.
 
 End specification.
 
 Section closed_proof.
   Context `{!heapGS Σ, !promiseGpreS Σ, !savedPredG Σ val}.
-  Context `{!ListLib Σ}.
 
   Lemma promiseInv_inner_init :
     ⊢ |==> ∃ _ : promiseGS Σ, promiseInv_inner.
@@ -1143,36 +1385,37 @@ Section closed_proof.
   Local Program Instance async_comp_lib `{!promiseGS Σ} :
     AsyncCompLib (Σ:=Σ) := {
     coop := Coop;
-    is_fiber_state := isFiberState;
-    fiber_context := fiberContext;
+    tlv_agree := tlvAgree;
+    tlv_agree_Persistent := _;
+    fiber_resources := fiberResources;
     is_promise := λ v Φ, (∃ (p : loc), ⌜ v = #p ⌝ ∗ isPromise p Φ)%I;
     is_promise_Persistent := _;
     promise_inv := promiseInv;
+    promise_inv_Persistent := _;
     get_context_spec := ewp_get_context;
+    yield_spec := ewp_yield;
   }.
   Next Obligation.
-   iIntros (????) "(HfCtx&HpInv&Hf)". 
-   iApply (ewp_mono with "[HfCtx HpInv Hf]").
+   iIntros (?????) "(HfRes&HpInv&Hf)". 
+   iApply (ewp_mono with "[HfRes HpInv Hf]").
    iApply ewp_fork_promise. iFrame.
    iIntros (?) "(%&->&H2&H3)".
    iModIntro.
    iFrame. iExists _. by iFrame.
   Qed.
   Next Obligation. 
-    iIntros (????) "(HfCtx & ? & % & -> & ?)". 
+    iIntros (?????) "(HfRes & ? & % & -> & ?)". 
     iApply ewp_await; iFrame. 
   Qed.
 
-  Theorem run_correct main : run_spec main.
+  Theorem run_correct init main (I Φ : val -> iProp Σ) : run_spec init main I Φ.
   Proof.
     rewrite /run_spec.
-    iIntros "He".
+    iIntros "Hinit He".
     iMod promiseInv_init as "[%HpromiseGS #HpInv]".
     iSpecialize ("He" $! async_comp_lib). iModIntro.
-    iApply (ewp_run _ (λ _, True)%I with "[HpInv He]").
+    iApply (ewp_run _ _ I Φ with "[HpInv He Hinit]").
     iFrame.
     by iAssumption.
   Qed.
 End closed_proof.
-
-Print Assumptions  run_correct.
