theories/language/neutral_contexts.v
@@ -62,7 +62,7 @@ Instance CaseCtx_neutral e1 e2 : NeutralFrame (CaseCtx e1 e2).
 Proof. constructor => m v k σ. by apply CaseEffS. Qed.
 Instance AllocNLCtx_neutral v2 : NeutralFrame (AllocNLCtx v2).
 Proof. constructor => m v k σ. by apply AllocNLEffS. Qed.
-Instance AllocCtx_neutral e1 : NeutralFrame (AllocNRCtx e1).
+Instance AllocNRCtx_neutral e1 : NeutralFrame (AllocNRCtx e1).
 Proof. constructor => m v k σ. by apply AllocNREffS. Qed.
 Instance LoadCtx_neutral : NeutralFrame LoadCtx.
 Proof. constructor => m v k σ. by apply LoadEffS. Qed.
